\subsection{End of chapter exercises}
\begin{exercise}{Neyman-Pearson Criterion}{exercise_4.1}
    The probability of error is not the only performance measure for binary classification. Indeed, the
    probability of error depends on the prior probability of the class label $Y$, and it may be that the
    frequency of the classes changes from training to testing data. In such cases, it is desirable to have a performance measure that does not require knowledge of the prior class probability. Let $P_y$ be the class conditional distribution of class $y\in\{0,1\}$. Define $R_y(h)=P_y(h(X) \ne y)$. Also let $\alpha \in (0,1)$. For $\mathcal{H}\subset\{0,1\}^{\mathcal{X}}$, define:

    \begin{align*}
        R^*_{\mathcal{H}, 1} &= \inf_{h\in\mathcal{H}} R_1(h) \\
        &\text{s.t. } R_0(h) \le \alpha 
    \end{align*}

    In this problem you will investigate a discrimination rule that is probably approximately correct with respect to the above criterion, which is sometimes called the Neyman-Pearson criterion based on connections to the Neyman-Pearson lemma in hypothesis testing.

    \noindent Suppose we observe $X_1^y, X_2^y, \dots, X_{n_y}^y \sim P_y$ for $y\in\{0,1\}$. Define the empirical errors:
    \begin{align*}
        \widehat{R_y}(h) = \frac{1}{n_y} \sum_{i=1}^{n_y} \1{h(X_i^y) \ne y}
    \end{align*}

    Fix $\epsilon > 0$ and consider the discrimination rule:
    \begin{align*}
        \widehat{h_n} &= \arg\min_{h\in\mathcal{H}} \widehat{R_1}(h) \\
        &\text{s.t. } \widehat{R_0}(h) \le \alpha + \frac{\epsilon}{2} 
    \end{align*}

    Suppose $\mathcal{H}$ is finite. Show that with high probability:
    \begin{align*}
        R_0(\widehat{h_n}) \le \alpha + \epsilon \text{ and } R_1(\widehat{h_n}) \le R^*_{\mathcal{H}, 1} + \epsilon
    \end{align*}
\end{exercise}

\begin{solution*}[Exercise \ref{ex:exercise_4.1}]
We will prove each point one by one:

\begin{itemize}
\item ${\bf (i)} \ R_0(\widehat{h_n}) \le \alpha + \epsilon$ \textbf{with high probability}. 

\begin{subproof}{\newline Claim 1 : $\forall y \in \{0,1\}, \epsilon>0 : P\biggRound{ \sup_{h\in\mathcal{H}} \biggAbs{ \widehat{R_y}(h) - R_y(h) } \ge \epsilon } \le 2|\mathcal{H}|e^{-2n\epsilon^2}$}
    We have that $n\widehat{R_n}(h)\sim Binomial(n, R_y(h))$ for all $h\in\mathcal{H}$. Hence, we have:
    \begin{align*}
        P\biggRound{
            \biggAbs{\widehat{R_y}(h) - R_y(h)} \ge \epsilon
        }
        &= 
        P\biggRound{
            \biggAbs{n\widehat{R_y}(h) - nR_y(h)} \ge n\epsilon
        } \\
        &= 
        P\biggRound{
            \biggAbs{n\widehat{R_y}(h) - \mathbb{E}\bigSquare{n\widehat{R_y}(h)}} \ge n\epsilon
        } \\
        &\le 
        2\exp\biggRound{
            -\frac{2n^2\epsilon^2}{n}
        } = 
        2e^{-2n\epsilon^2} \ \ \ (\text{Hoeffding's inequality})
    \end{align*}

    \noindent From the above, we have:
    \begin{align*}
        P\biggRound{
            \sup_{h\in\mathcal{H}} \biggAbs{
                \widehat{R_y}(h) - R_y(h)
            } \ge \epsilon
        } 
        &= 
        P\biggRound{
            \bigcup_{h\in\mathcal{H}} \biggCurl{ \bigAbs{
                \widehat{R_y}(h) - R_y(h)
            } \ge \epsilon
        } } \\
        &\le 
        \sum_{h\in\mathcal{H}} P\biggRound{ 
            \bigAbs{
                \widehat{R_y}(h) - R_y(h)
            } \ge \epsilon
        } \\
        &\le
        \sum_{h\in\mathcal{H}} 2e^{-2n\epsilon^2} = 2|\mathcal{H}|e^{-2n\epsilon^2}
    \end{align*}
\end{subproof}

\noindent\newline From the assumption, we have:
\begin{align*}
    \widehat{R_0}(\widehat{h_n}) \le \alpha + \frac{\epsilon}{2}
\end{align*}

\noindent Hence, we have:
\begin{align*}
    R_0(\widehat{h_n})
        &= \widehat{R_0}(\widehat{h_n}) + R_0(\widehat{h_n}) - \widehat{R_0}(\widehat{h_n}) \\
        &\le \alpha + \frac{\epsilon}{2} + \bigAbs{R_0(\widehat{h_n}) - \widehat{R_0}(\widehat{h_n})} \\
        &\le \alpha + \frac{\epsilon}{2} + \sup_{h\in\mathcal{H}}\bigAbs{
            R_0(\widehat{h_n}) - \widehat{R_0}(\widehat{h_n})
        }
\end{align*}

\noindent From \textbf{Claim 1}, we know that:
\begin{align*}
    P\biggRound{
        \sup_{h\in\mathcal{H}} \biggAbs{
            R_0(h) - \widehat{R_0}(h)
        } \ge\frac{\epsilon}{2}
    } &\le 2|\mathcal{H}|e^{-n\epsilon^2/2} \\
    \implies
    P\biggRound{
        \sup_{h\in\mathcal{H}} \biggAbs{
            R_0(h) - \widehat{R_0}(h)
        } \le\frac{\epsilon}{2}
    } &\ge 1 - 2|\mathcal{H}|e^{-n\epsilon^2/2} 
\end{align*}

\noindent Hence, with probability of at least $1 - 2|\mathcal{H}|e^{-n\epsilon^2/2}$, we have:
\begin{align*}
    R_0(\widehat{h_n}) \le \alpha + \frac{\epsilon}{2} + \frac{\epsilon}{2} = \alpha + \epsilon
\end{align*}

\item ${\bf (ii)} \ R_1(\widehat{h_n}) \le R_{\mathcal{H}, 1}^* + \epsilon \textbf{ with high probability}$.

\begin{subproof}{\newline Claim 2 : $R_1(\widehat{h_n}) - R_{\mathcal{H},1}^* \le 2\sup_{h\in\mathcal{H}}\bigAbs{\widehat{R_1}(h) - R_1(h)}$}
    Let $h' \in \mathcal{H}$ be any function such that $\widehat{R_0}(h') \le \alpha + \frac{\epsilon}{2}$. We have:
    \begin{align*}
        R_1(\widehat{h_n}) - R^*_{\mathcal{H},1}
            &= R_1(\widehat{h_n}) - \widehat{R_1}(\widehat{h_n}) 
             + \widehat{R_1}(\widehat{h_n}) - \widehat{R_1}(h')
             + \widehat{R_1}(h') - R^*_{\mathcal{H}, 1} \\
            &\le \bigAbs{R_1(\widehat{h_n}) - \widehat{R_1}(\widehat{h_n})}
                + \underbrace{\widehat{R_1}(\widehat{h_n}) - \widehat{R_1}(h')}_{\le 0}
                + \bigAbs{\widehat{R_1}(h') - R^*_{\mathcal{H}, 1}} \\
            &\le \bigAbs{R_1(\widehat{h_n}) - \widehat{R_1}(\widehat{h_n})}
            + \bigAbs{\widehat{R_1}(h') - R^*_{\mathcal{H}, 1}} \\
            &\le 2\sup_{h\in\mathcal{H}} \bigAbs{
                \widehat{R_1}(h) - R_1(h) 
            }
    \end{align*}
\end{subproof}

\noindent From \textbf{Claim 2}, we have:
\begin{align*}
    P\bigRound{
        R_1(\widehat{h_n}) - R^*_{\mathcal{H}, 1} \ge \epsilon
    } 
    &\le
    P\bigRound{
        2\sup_{h\in\mathcal{H}} \bigAbs{
            \widehat{R_1}(h) - R_1(h) 
        } \ge \epsilon
    }  \\
    &= P\bigRound{
        \sup_{h\in\mathcal{H}} \bigAbs{
            \widehat{R_1}(h) - R_1(h) 
        } \ge \frac{\epsilon}{2}
    }  \\
    &\le 2|\mathcal{H}|e^{-n\epsilon^2/2} \ \ \ (\text{From }\textbf{Claim 1}) \\
    \implies 
    P\bigRound{
        R_1(\widehat{h_n}) - R^*_{\mathcal{H}, 1} \le \epsilon
    } &\ge 1 - 2|\mathcal{H}|e^{-n\epsilon^2/2} 
\end{align*}

\noindent Hence, with probability of at least $1 - 2|\mathcal{H}|e^{-n\epsilon^2/2}$, we have that $R_1(\widehat{h_n}) \le R^*_{\mathcal{H}, 1} + \epsilon$.

\end{itemize}
\end{solution*}